What with the change to REDUCE_ss and new_specification, I've just copied across my versions of these files from my independent attempt to formalise Hankin's book on the lambda calculus.  The main loss is the proof that the length function exists, because I have code that does this automatically.

examples/lambda/ncScript.sml
@@ -17,10 +17,6 @@ struct
 open HolKernel Parse boolLib
      bossLib arithmeticTheory pred_setTheory dBTheory;
 
-infixr 3 -->;
-infix && ## |-> THEN THENL THENC ORELSE ORELSEC THEN_TCL ORELSE_TCL;
-infix 8 by;
-
 val _ = new_theory "nc";
 
 
@@ -234,11 +230,7 @@ STRIP_ASSUME_TAC WRAP_DB_EXISTS
   THEN RW_TAC OK_ss [lemma,LAM,SUB_DEF,VARR]);
 
 
-val ABS =
-  new_specification
-    {name = "ABS_DEF",
-     consts = [{const_name = "ABS", fixity = Prefix}],
-     sat_thm = ABS_EXISTS};
+val ABS = new_specification ("ABS_DEF", ["ABS"], ABS_EXISTS);
 
 (* ********************************************************************* *)
 (* End of characterization.                                              *)
@@ -511,10 +503,7 @@ val BODY_DEF =
       `?f:'a nc -> (string->'a nc). !x u. f(LAM x ^u) = \y. [VAR y/x]u`,
       STRIP_ASSUME_TAC th2 THEN Q.EXISTS_TAC `hom` THEN RW_TAC std_ss [])
  in
-    new_specification
-       {name = "BODY_DEF",
-        consts = [{const_name="BODY", fixity=Prefix}],
-        sat_thm = lemma}
+    new_specification ("BODY_DEF", ["BODY"], lemma)
  end;
 
 (* --------------------------------------------------------------------- *)
@@ -705,13 +694,21 @@ nc_INDUCT_TAC
 
 
 (* ===================================================================== *)
-(* Andy's injectivity theorems                                           *)
+(* Injectivity theorems                                                  *)
 (* ===================================================================== *)
 
 val INJECTIVITY_LEMMA1 = Q.store_thm("INJECTIVITY_LEMMA1",
 `!x u x1 u1.
    (LAM x u = LAM x1 u1) ==> (u = [VAR x/x1]u1)`,
 PROVE_TAC [nc_INJECTIVITY,lemma14a]);
+
+val LAM_VAR_INJECTIVE = store_thm(
+  "LAM_VAR_INJECTIVE",
+  ``!x b1 b2. (LAM x b1 = LAM x b2) = (b1 = b2)``,
+  REPEAT GEN_TAC THEN EQ_TAC THEN SIMP_TAC std_ss [] THEN STRIP_TAC THEN
+  IMP_RES_THEN SUBST_ALL_TAC INJECTIVITY_LEMMA1 THEN
+  SIMP_TAC std_ss [lemma14a]);
+
 
 val lemma =
  REWRITE_RULE [IN_UNION,IN_SING,DE_MORGAN_THM,IN_INSERT]
@@ -872,11 +869,7 @@ Q.EXISTS_TAC `\lam t. let x = @x. ~(x IN (FV lam)) in [t/x](BODY lam x)`
    THEN STRIP_ASSUME_TAC (SPEC_ALL lemma)
    THEN RW_TAC std_ss [lemma15a,lemma14a]);
 
-val BETA =
-  new_specification
-  {name    = "BETA_DEF",
-   consts  = [{fixity = Prefix, const_name = "BETA"}],
-   sat_thm = BETA_EXISTS};
+val BETA = new_specification ("BETA_DEF", ["BETA"], BETA_EXISTS);
 
 (* --------------------------------------------------------------------- *)
 (* BODY is definable given BETA.                                         *)
@@ -896,7 +889,7 @@ Q.EXISTS_TAC `\u y. BETA u (VAR y)` THEN RW_TAC std_ss [BETA]);
 (*       FVS [(t1,x1),...,(tn,xn)] = FV t1 UNION ... UNION FV tn         *)
 (* --------------------------------------------------------------------- *)
 
-val ISUB_DEF =
+val ISUB_def =
  Define
      `($ISUB t [] = t)
   /\  ($ISUB t ((s,x)::rst) = $ISUB ([s/x]t) rst)`;
@@ -955,6 +948,45 @@ HO_MATCH_MP_TAC RENAMING_IND
    THEN RW_TAC list_ss []
    THEN PROVE_TAC [RENAMING_CASES]);
 
+(* ----------------------------------------------------------------------
+    Simple properties of ISUB
+   ---------------------------------------------------------------------- *)
+
+val SUB_ISUB_SINGLETON = store_thm(
+  "SUB_ISUB_SINGLETON",
+  ``!t x u. [t/x]u = u ISUB [(t,x)]``,
+  SRW_TAC [][ISUB_def]);
+
+val ISUB_APPEND = store_thm(
+  "ISUB_APPEND",
+  ``!R1 R2 t. (t ISUB R1) ISUB R2 = t ISUB (APPEND R1 R2)``,
+  Induct THEN
+  ASM_SIMP_TAC (srw_ss()) [pairTheory.FORALL_PROD, ISUB_def]);
+
+(* ----------------------------------------------------------------------
+    ... and of RENAMING
+   ---------------------------------------------------------------------- *)
+
+val _ = temp_type_abbrev("renaming", ``:('a nc # string) list``)
+val RENAMING_THM = store_thm(
+  "RENAMING_THM",
+  ``RENAMING ([]:'a renaming) /\
+    (!(R:'a renaming) h.
+       RENAMING (h::R) = RENAMING R /\ ?y x. h = (VAR y,x)) /\
+    (!R1 R2:'a renaming.
+       RENAMING (APPEND R1 R2) = RENAMING R1 /\ RENAMING R2)``,
+  Q.SUBGOAL_THEN
+    `RENAMING ([]:'a renaming) /\
+    (!R:'a renaming h.
+       RENAMING (h::R) = RENAMING R /\ ?y x. h = (VAR y,x))`
+    (fn th => STRIP_ASSUME_TAC th THEN ASM_REWRITE_TAC [])
+  THENL [
+    SIMP_TAC (srw_ss()) [RENAMING_DEF] THEN REPEAT GEN_TAC THEN
+    CONV_TAC (LAND_CONV (REWR_CONV RENAMING_CASES)) THEN SRW_TAC [][] THEN
+    PROVE_TAC [],
+    Induct THEN SRW_TAC [][] THEN PROVE_TAC []
+  ]);
+
 
 (* --------------------------------------------------------------------- *)
 (* Interaction of ISUB with syntax constructors.                         *)
@@ -973,18 +1005,18 @@ val ISUB_VAR_RENAME = Q.store_thm("ISUB_VAR_RENAME",
         ==>
       !x. (VAR x) ISUB ss = VAR (RENAME ss x)`,
 HO_MATCH_MP_TAC RENAMING_IND
-  THEN RW_TAC std_ss [ISUB_DEF, RENAME_DEF, VNAME_DEF, SUB_VAR]
+  THEN RW_TAC std_ss [ISUB_def, RENAME_DEF, VNAME_DEF, SUB_VAR]
   THEN RW_TAC std_ss []);
 
 val ISUB_CON = Q.store_thm("ISUB_CON",
 `!^R k. (CON k) ISUB ^R = CON k`,
 Induct THEN Ho_Rewrite.REWRITE_TAC[pairTheory.FORALL_PROD]
- THEN RW_TAC std_ss [ISUB_DEF, SUB_THM]);
+ THEN RW_TAC std_ss [ISUB_def, SUB_THM]);
 
 val ISUB_APP = Q.store_thm("ISUB_APP",
 `!^R t u. (t @@ u) ISUB ^R = (t ISUB ^R) @@ (u ISUB ^R)`,
 Induct THEN Ho_Rewrite.REWRITE_TAC[pairTheory.FORALL_PROD]
-  THEN RW_TAC std_ss [ISUB_DEF, SUB_THM]);
+  THEN RW_TAC std_ss [ISUB_def, SUB_THM]);
 
 val ISUB_LAM = Q.store_thm("ISUB_LAM",
 `!^R x. ~(x IN (DOM ^R UNION FVS ^R))
@@ -994,94 +1026,23 @@ Induct THENL
  [ALL_TAC, Ho_Rewrite.REWRITE_TAC[pairTheory.FORALL_PROD]
            THEN Cases_on `x` THEN POP_ASSUM MP_TAC]
  THEN RW_TAC list_ss
- [ISUB_DEF,DOM_DEF,FVS_DEF,FV_THM,IN_UNION,IN_SING,DE_MORGAN_THM,SUB_THM]);
+ [ISUB_def,DOM_DEF,FVS_DEF,FV_THM,IN_UNION,IN_SING,DE_MORGAN_THM,SUB_THM]);
 
-(* --------------------------------------------------------------------- *)
-(* Definition of length -- set-based construction.                       *)
-(* --------------------------------------------------------------------- *)
-
-val existence =
- let val instth = INST_TYPE [beta |-> Type`:num`] nc_RECURSION
-     val con = `\x. 1` and
-         var = `\x. 1` and
-         app = `\n m t u. (n + m)` and
-         lam = `\f g. let v = NEW(FV(ABS g)) in (f v) + 1`
-     val th1 = BETA_RULE (Q.SPECL [con,var,app,lam] instth)
-     val th2 = BETA_RULE (CONJUNCT1 (CONV_RULE EXISTS_UNIQUE_CONV th1))
- in
-   REWRITE_RULE [ABS] th2
- end;
-
-local val def = body(rand(concl existence))
-in
-val vlemma = Q.prove(
-`^def ==> !x y z. hom([VAR y/z](VAR x)) = 1`,
-RW_TAC std_ss [] THEN Cases_on `z:string = x`
- THEN RW_TAC std_ss [SUB_THM])
-end;
-
-val lemma1 = Q.prove(
-`!ss u t x. [t/x](u ISUB ss) = u ISUB (APPEND ss [(t,x)])`,
-Induct THEN Ho_Rewrite.REWRITE_TAC[pairTheory.FORALL_PROD]
-   THEN RW_TAC list_ss [ISUB_DEF]);
-
-val lemma2 = Q.prove(
-`[a/b]([x/y]u) = u ISUB [(x,y);(a,b)]`,
-RW_TAC std_ss [ISUB_DEF]);
+val _ = BasicProvers.export_rewrites ["FV_THM", "nc_DISTINCT",
+                                      "nc_INJECTIVITY", "LAM_VAR_INJECTIVE"];
 
 
-local val (hom,def) = dest_exists(concl existence)
-in
-val lemma3 = Q.prove(
-`^def ==> !u ss. RENAMING ss ==> (^hom (u ISUB ss) = ^hom u)`,
-STRIP_TAC THEN nc_INDUCT_TAC2 THENL
- [RW_TAC std_ss [ISUB_CON],
-  RW_TAC std_ss [ISUB_VAR_RENAME],
-  RW_TAC std_ss [ISUB_APP],
-  Q.EXISTS_TAC `{}`
-    THEN REWRITE_TAC [FINITE_EMPTY,NOT_IN_EMPTY]
-    THEN REPEAT STRIP_TAC THEN
-    let val vs = Term`(DOM ss) UNION (FVS (ss:('a nc # string) list))
-                               UNION (FV (u:'a nc))`
-        val th1 = Q.prove(`FINITE ^vs`,
-                  REWRITE_TAC [FINITE_UNION,FINITE_FV, FINITE_FVS,FINITE_DOM])
-        val th2 = MATCH_MP NEW_FRESH_string th1
-        val th3 = REWRITE_RULE [UNION_ASSOC] th2
-        val th4 = PURE_ONCE_REWRITE_RULE [IN_UNION] th3
-        val th5 = REWRITE_RULE [GSYM UNION_ASSOC,DE_MORGAN_THM] th4
-        val th6 = MATCH_MP SIMPLE_ALPHA (CONJUNCT2 th5)
-    in
-      SUBST1_TAC (Q.SPEC `y` th6)
-       THEN ASM_REWRITE_TAC [MATCH_MP ISUB_LAM (CONJUNCT1 th5)]
-    end
-    THEN REWRITE_TAC [lemma1,lemma2,GSYM (CONJUNCT2 ISUB_DEF)]
-    THEN CONV_TAC (DEPTH_CONV pairLib.let_CONV)
-    THEN REWRITE_TAC [GSYM ADD1] THEN AP_TERM_TAC
-    THEN REWRITE_TAC [lemma1,lemma2,GSYM (CONJUNCT2 ISUB_DEF)]
-    THEN (fn (A,g) =>
-            let val (lhs,rhs) = dest_eq g
-                val eq1 = mk_eq(lhs, Term`^hom u`)
-                and eq2 = mk_eq(rhs, Term`^hom u`)
-            in
-              SUBGOAL_THEN (mk_conj(eq1, eq2))
-                  (fn th => REWRITE_TAC [th]) (A,g)
-            end)
-     THEN PROVE_TAC [RENAMING_CASES,RENAMING_LEMMA]])
-  end;
+val NEW_ELIM_RULE = store_thm(
+  "NEW_ELIM_RULE",
+  ``!P X. FINITE X /\ (!v:string. ~(v IN X) ==> P v) ==>
+          P (NEW X)``,
+  PROVE_TAC [dBTheory.NEW_FRESH_string]);
 
-val lemma4 = Q.prove(`!x y. RENAMING [VAR x,y]`, PROVE_TAC[RENAMING_CASES]);
-val lemma5 = Q.prove(`[x/y]u = u ISUB [(x,y)]`,  REWRITE_TAC [ISUB_DEF]);
-
-val ncLENGTH_EXISTS = Q.store_thm("ncLENGTH_EXISTS",
-`?hom:'a nc->num.
-     (!k. hom(CON k) = 1) /\
-     (!x. hom(VAR x) = 1) /\
-     (!t u. hom(t @@ u) = (hom t) + (hom u)) /\
-     (!x u. hom(LAM x u) = SUC (hom u))`,
-STRIP_ASSUME_TAC existence
-  THEN IMP_RES_TAC lemma3
-  THEN Q.EXISTS_TAC `hom`
-  THEN RW_TAC std_ss [GSYM ADD1,lemma4,lemma5]);
+val NEW_ELIM_RULE_SUBSET = store_thm(
+  "NEW_ELIM_RULE_SUBSET",
+  ``!P X Y. FINITE X /\ Y SUBSET X /\ (!v:string. ~(v IN Y) ==> P v) ==>
+            P (NEW X)``,
+  PROVE_TAC [dBTheory.NEW_FRESH_string, pred_setTheory.SUBSET_DEF]);
 
 
 val _ = export_theory();
